test/SemanticsCCS.lean
@@ -1,0 +1,13 @@
+
+
+def firecracker : CCS0 :=
+  (Action.mk ("light")) . (Action.mk "bang") . nil
+
+def defective_firecracker : CCS0 :=
+  (Action.mk "light") . (Action.mk "τ") . nil
+
+def possibly_defective_firecracker : CCS0 :=
+  CCS0.prefix (act "light")
+    (CCS0.choice
+      (CCS0.prefix (act "τ") CCS0.null)
+      (CCS0.prefix (act "bang") CCS0.null))
